src/Dafny/examples/fs/mem_dirent.dfy
@@ -1,0 +1,227 @@
+include "dirent.dfy"
+
+module MemDirEntries
+{
+  import opened Std
+  import opened DirEntries
+  import opened Machine
+  import opened ByteSlice
+  import opened FsKinds
+  import IntEncoding
+
+  datatype MemDirEnt = MemDirEnt(name: Bytes, ino: Ino)
+  {
+    function val(): DirEnt
+      reads name
+      requires Valid()
+    {
+      DirEnt(name.data, ino)
+    }
+
+    predicate Valid()
+      reads name
+    {
+      && is_pathc(name.data)
+    }
+  }
+
+  method NullTerminatedEqualSmaller(bs1: Bytes, bs2: Bytes) returns (p:bool)
+    requires bs1.Valid() && bs2.Valid()
+    requires bs1.Len() <= bs2.Len()
+    ensures p == (decode_null_terminated(bs1.data) == decode_null_terminated(bs2.data))
+  {
+    var i: uint64 := 0;
+    var len: uint64 := bs1.Len();
+    while i < len
+      invariant 0 <= i as nat <= |bs1.data|
+      invariant bs1.data[..i] == bs2.data[..i]
+      invariant decode_null_terminated(bs1.data) == bs1.data[..i] + decode_null_terminated(bs1.data[i..])
+      invariant decode_null_terminated(bs2.data) == bs2.data[..i] + decode_null_terminated(bs2.data[i..])
+
+    {
+      var b1 := bs1.Get(i);
+      var b2 := bs2.Get(i);
+      if b1 == 0 || b2 == 0 {
+        return b1 == b2;
+      }
+      assert b1 != 0 && b2 != 0;
+      if b1 != b2 {
+        assert decode_null_terminated(bs1.data)[i] == b1;
+        assert decode_null_terminated(bs2.data)[i] == b2;
+        return false;
+      }
+      i := i + 1;
+    }
+    if bs1.Len() == bs2.Len() {
+      return true;
+    }
+    assert bs1.Len() < bs2.Len();
+    var last := bs2.Get(bs1.Len());
+    return last == 0;
+  }
+
+  method NullTerminatedEqual(bs1: Bytes, bs2: Bytes) returns (p:bool)
+    requires bs1.Valid() && bs2.Valid()
+    ensures p == (decode_null_terminated(bs1.data) == decode_null_terminated(bs2.data))
+  {
+    if bs1.Len() <= bs2.Len() {
+      p := NullTerminatedEqualSmaller(bs1, bs2);
+      return;
+    }
+    p := NullTerminatedEqualSmaller(bs2, bs1);
+    return;
+  }
+
+  class MemDirents
+  {
+    ghost var val: Dirents
+    const bs: Bytes
+
+    ghost const Repr: set<object> := {this, bs}
+
+    predicate Valid()
+      reads Repr
+    {
+      && bs.data == val.enc()
+      && |bs.data| == 4096
+    }
+
+    constructor(bs: Bytes, ghost dents: Dirents)
+      requires bs.data == dents.enc()
+      ensures Valid()
+      ensures val == dents
+    {
+      this.bs := bs;
+      this.val := dents;
+      new;
+      val.enc_len();
+    }
+
+    lemma data_one(k: nat)
+      requires Valid()
+      requires k < 128
+      ensures bs.data[k*32..(k+1) * 32] == val.s[k].enc()
+    {
+      C.concat_homogeneous_one_list(C.seq_fmap(Dirents.encOne, val.s), k, 32);
+    }
+
+    lemma data_one_ino(k: nat)
+      requires Valid()
+      requires k < 128
+      ensures bs.data[k*32 + 24..k*32 + 32] == IntEncoding.le_enc64(val.s[k].ino)
+    {
+      data_one(k);
+      val.s[k].enc_app();
+      assert bs.data[k*32..(k+1)*32][24..32] == bs.data[k*32 + 24..k*32 + 32];
+    }
+
+    method get_ino(k: uint64) returns (ino: Ino)
+      requires Valid()
+      requires k < 128
+      ensures ino == val.s[k].ino
+    {
+      // we'll prove it's an Ino later, for now it's just a uint64
+      var ino': uint64 := IntEncoding.UInt64Get(bs, k*32 + 24);
+      data_one_ino(k as nat);
+      IntEncoding.lemma_le_enc_dec64(val.s[k].ino);
+      ino := ino';
+    }
+
+    method get_name(k: uint64) returns (name: Bytes)
+      requires Valid()
+      requires k < 128
+      ensures fresh(name) && name.Valid() && |name.data| == 24
+      ensures encode_pathc(val.s[k].name) == name.data
+    {
+      name := NewBytes(24);
+      name.CopyFrom(bs, k*32, 24);
+      data_one(k as nat);
+      val.s[k].enc_app();
+      assert bs.data[k*32..(k+1)*32][..24] == bs.data[k*32..k*32 + 24];
+    }
+
+    method is_used(k: uint64) returns (p:bool)
+      requires Valid()
+      requires k < 128
+      ensures p == val.s[k].used()
+    {
+      var ino := get_ino(k);
+      p := ino != 0;
+    }
+
+    method is_name(k: uint64, needle: Bytes) returns (r:Option<Ino>)
+      requires Valid()
+      requires k < 128
+      requires needle.Valid()
+      requires is_pathc(needle.data)
+      ensures r.None? ==> !(val.s[k].used() && val.s[k].name == needle.data)
+      ensures r.Some? ==> val.s[k].used() && val.s[k].name == needle.data && val.s[k].ino == r.x
+    {
+      var ino := get_ino(k);
+      if ino == 0 {
+        return None;
+      }
+      var name := get_name(k);
+      assert decode_null_terminated(name.data) == val.s[k].name by {
+        decode_encode(val.s[k].name);
+      }
+      decode_nullterm_no_null(needle.data);
+      var equal := NullTerminatedEqualSmaller(needle, name);
+      if equal {
+        return Some(ino);
+      } else {
+        return None;
+      }
+    }
+
+    method findFree() returns (free_i: uint64)
+      requires Valid()
+      ensures free_i as nat == val.findFree()
+    {
+      var i: uint64 := 0;
+      while i < 128
+        invariant 0 <= i as nat <= 128
+        invariant forall k:nat | k < i as nat :: val.s[k].used()
+      {
+        var p := is_used(i);
+        if !p {
+          C.find_first_characterization(Dirents.is_unused, val.s, i as nat);
+          return i;
+        }
+        i := i + 1;
+      }
+      C.find_first_characterization(Dirents.is_unused, val.s, 128);
+      return 128;
+    }
+
+    method findName(name: Bytes) returns (r: Option<(uint64, Ino)>)
+      requires Valid()
+      requires name.Valid() && is_pathc(name.data)
+      ensures r.None? ==> name.data !in val.dir
+      ensures r.Some? ==>
+      && name.data in val.dir
+      && r.x.0 < 128
+      && r.x.0 as nat == val.findName(name.data)
+      && val.dir[name.data] == r.x.1
+    {
+      ghost var p: PathComp := name.data;
+      var i: uint64 := 0;
+      while i < 128
+        invariant 0 <= i as nat <= 128
+        invariant forall k:nat | k < i as nat :: !(val.s[k].used() && val.s[k].name == p)
+      {
+        var ino := is_name(i, name);
+        if ino.Some? {
+          C.find_first_characterization(preDirents.findName_pred(p), val.s, i as nat);
+          assert val.findName(p) == i as nat;
+          val.findName_found(p);
+          return Some( (i, ino.x) );
+        }
+        i := i + 1;
+      }
+      C.find_first_characterization(preDirents.findName_pred(p), val.s, 128);
+      val.findName_not_found(p);
+      return None;
+    }
+  }
+}
